\documentclass[10pt, a4paper,twocolumn]{article}
    \author{ianaesthetic}
    \title{3d Game Programming with DirectX 11}
\usepackage{indentfirst, amsmath, fontspec, listings, xcolor, amssymb}
%\usepackage{verbatim}

\usepackage{xeCJK}
\setCJKmainfont{Microsoft YaHei}

\newfontfamily\consolas{Consolas}
\lstset{numberstyle = \small\consolas, basicstyle=\small\consolas}

\XeTeXlinebreaklocale "zh"
\XeTeXlinebreakskip = 0pt plus 1pt

\begin{document}
    胡博闻 2016121518 
    \medskip 

    49. 
    $$
        P(2X + 1 = k) = 
        \begin{cases}
            0.1, & k = -1 \\
            0.2, & k = 1 \\
            0.3, & k = 3 \\
            0.4, & k = 5
        \end{cases}
    $$

    $$
        p(X^2 = k) = 
        \begin{cases}
            0.2, & k = 0 \\ 
            0.4, & k = 1 \\
            0.4, & k = 4 
        \end{cases}
    $$

    50.
    $$F(x) = 
        \begin{cases}
            0 & x \leqslant 0 \\
        1 - e^{-x}  & x > 0
        \end{cases}
    $$

    $$
        \begin{aligned}
            G(y)
            &= P(Y \leqslant y) \\
            &= P(X^2 \leqslant y) \\
            &= P(X \leqslant \sqrt{y}) \\
            &= F(\sqrt{y})  
        \end{aligned}
    $$

    $$
        G(y) = 
        \begin{cases}
            0 & y \leqslant 0 \\ 
            1 - e^{-\sqrt{y}} & y > 0 
        \end{cases}
    $$

    $$
        P(Y) = 
        \begin{cases}
            \frac{\sqrt{y}e^{-\sqrt{y}}}{2y} & y >  0 \\
            0 & y \leqslant 0 
        \end{cases}
    $$

    55. 
    $$
        p(x) = 
        \begin{cases}
            \frac{1}{2\pi} & x \in [0, 2\pi] \\
            0 & x \notin  [0, 2\pi]
        \end{cases}
    $$

    $$
        F(x) = 
        \begin{cases}
            0 & x \in (-\infty, 0) \\
            \frac{x}{2\pi} & x \in [0, 2\pi] \\
            1 & x \in (2, +\infty)
        \end{cases}
    $$

    $$
        \begin{aligned}
            G(y) &= P(Y \leqslant y) \\
                &= P(cosX \leqslant y) \\ 
                &= P(\text{arccos}y \leqslant X \leqslant 2\pi - \text{arccos}y)
        \end{aligned}
    $$

    $$
        G(y) = 
        \begin{cases}
            0 & y \in (-\infty, -1) \\
            1 - \frac{\text{arccos}y}{\pi} & y \in [-1, 1] \\ 
            1 & y \in (1, +\infty)
        \end{cases}
    $$

    $$
        p(y) = 
        \begin{cases}
            \frac{1}{\pi\sqrt{1 - y^2}} & y \in [-1, 1] \\
            0 & y \notin [-1, 1]
        \end{cases}
    $$

\end{document}